mppa_k1c/Asmblockdeps.v
@@ -846,7 +846,7 @@ Theorem bisimu_par_wio_basic ge fn rsr rsw mr mw sr sw bi:
   Ge = Genv ge fn ->
   match_states (State rsr mr) sr ->
   match_states (State rsw mw) sw ->
-  match_outcome (parexec_basic_instr ge bi rsr rsw mr mw) (inst_prun Ge (trans_basic bi) sw sr sr).
+  match_outcome (bstep ge bi rsr rsw mr mw) (inst_prun Ge (trans_basic bi) sw sr sr).
 Proof.
 
 (* a little tactic to automate reasoning on preg_eq *)
@@ -1004,7 +1004,7 @@ Proof.
   induction bdy as [|i bdy]; simpl; eauto. 
   intros.
   exploit (bisimu_par_wio_basic ge fn rsr rsw mr mw sr sw i); eauto.
-  destruct (parexec_basic_instr _ _ _ _ _ _); simpl.
+  destruct (bstep _ _ _ _ _ _); simpl.
   - intros (s' & X1 & X2). rewrite X1; simpl; eauto.
   - intros X; rewrite X; simpl; auto.
 Qed.
@@ -1015,7 +1015,7 @@ Theorem bisimu_par_control ex sz aux ge fn rsr rsw mr mw sr sw:
   match_states (State rsw mw) sw ->
   match_outcome (parexec_control ge fn ex (incrPC (Ptrofs.repr sz) rsr) (rsw#PC <- aux) mw) (inst_prun Ge (trans_pcincr sz (trans_exit ex)) sw sr sr).
 Proof.
-  intros GENV MSR MSW; unfold parexec_exit.
+  intros GENV MSR MSW; unfold estep.
   simpl in *. inv MSR. inv MSW.
   destruct ex.
   - destruct c; destruct i; try discriminate; simpl.
@@ -1071,9 +1071,9 @@ Theorem bisimu_par_exit ex sz ge fn rsr rsw mr mw sr sw:
   Ge = Genv ge fn ->
   match_states (State rsr mr) sr ->
   match_states (State rsw mw) sw ->
-  match_outcome (parexec_exit ge fn ex (Ptrofs.repr sz) rsr rsw mw) (inst_prun Ge (trans_pcincr sz (trans_exit ex)) sw sr sr).
+  match_outcome (estep ge fn ex (Ptrofs.repr sz) rsr rsw mw) (inst_prun Ge (trans_pcincr sz (trans_exit ex)) sw sr sr).
 Proof.
-  intros; unfold parexec_exit.
+  intros; unfold estep.
   exploit (bisimu_par_control ex sz rsw#PC ge fn rsr rsw mr mw sr sw); eauto.
   cutrewrite (rsw # PC <- (rsw PC) = rsw); auto.
   apply extensionality. intros; destruct x; simpl; auto.
