mppa_k1c/PostpassSchedulingproof.v
@@ -240,7 +240,7 @@ Lemma exec_basic_instr_pc_var:
   exec_basic_instr ge i rs m = Next rs' m' ->
   exec_basic_instr ge i (rs # PC <- v) m = Next (rs' # PC <- v) m'.
 Proof.
-  intros. unfold exec_basic_instr in *. unfold parexec_basic_instr in *. destruct i.
+  intros. unfold exec_basic_instr in *. unfold bstep in *. destruct i.
   - unfold exec_arith_instr in *. destruct i; destruct i.
       all: try (exploreInst; inv H; apply next_eq; auto;
       apply functional_extensionality; intros; rewrite regset_double_set; auto; discriminate).
@@ -681,7 +681,7 @@ Lemma transf_exec_basic_instr:
   forall i rs m, exec_basic_instr ge i rs m = exec_basic_instr tge i rs m.
 Proof.
   intros. pose symbol_address_preserved.
-  unfold exec_basic_instr. unfold parexec_basic_instr. exploreInst; simpl; auto; try congruence.
+  unfold exec_basic_instr. unfold bstep. exploreInst; simpl; auto; try congruence.
   unfold parexec_arith_instr; unfold arith_eval_r; exploreInst; simpl; auto; try congruence.
 Qed.
 
